Update qTESLA spec to v2.3 of 10/31/2018
Some changes to the spec were already incorporated resulting from
discussions with Patrick. Major change is using the hash of the
message as input to hash H, as part of signature generation and
validation, instead of the full message body.

Also, move instantiations of various XOFs and other functions into
parameter sets; we were incorrectly using (c)SHAKE128 in a couple
places we should have been using the -256 versions. Parameterized
functions are now called from the spec.

Manually verified that the spec type-checks across all parameter sets,
and made changes or added refinements where necessary in order for this
to happen.

qtesla/spec/Spec.QTesla.fst
@@ -15,7 +15,7 @@ module Loops = Lib.LoopCombinators
 module Seq = Lib.Sequence
 module FSeq = FStar.Seq
 
-#reset-options "--z3rlimit 50 --max_fuel 0 --max_ifuel 1"
+#reset-options "--z3rlimit 80 --max_fuel 0 --max_ifuel 1"
 
 (** qTesla often uses [pos] as a variable name, so we define a transparent synonym *)
 unfold let positive = pos
@@ -199,7 +199,7 @@ let checkE e = poly_max_sum e params_h <= params_Le
 
 // Given an input pre-seed of \kappa bytes, return a buffer of (\kappa * ((k+3)/8)) bytes extended by the XOF
 val prf1: lbytes params_kappa -> lbytes (params_kappa * (params_k+3))
-let prf1 preseed = params_xof params_kappa preseed (params_kappa * (params_k+3))
+let prf1 preseed = params_prf1 params_kappa preseed (params_kappa * (params_k+3))
 
 val prf2: 
     #mLen:size_nat{mLen < max_size_t - 2 * params_kappa} 
@@ -209,27 +209,12 @@ val prf2:
   -> lbytes params_kappa
 let prf2 #mLen seedY r m =
   let concatenation = Seq.concat (Seq.concat seedY r) m in
-  params_xof (Seq.length concatenation) concatenation params_kappa
-
-// qTESLA's spec uses natural numbers that it increments as nonces for
-// cSHAKE, but the implementation takes uint16s. Instead of junking the
-// spec up with statements about the nonces staying within the range of
-// a uint16, we encapulsate it here.
-val cshake128_qtesla:
-    input_len:size_nat
-  -> input:lbytes input_len
-  -> nonce:nat
-  -> output_len:size_nat
-  -> lbytes output_len
-let cshake128_qtesla input_len input nonce output_len =
-  assume(nonce < maxint U16);
-  let cstm = u16 nonce in
-  cshake128_frodo input_len input cstm output_len
+  params_prf2 (Seq.length concatenation) concatenation params_kappa
 
 val genA_getC: 
     cBuf:bytes{Seq.length cBuf < max_size_t} 
   -> cPos:size_nat{(cPos+1) * computed_b <= Seq.length cBuf} 
-  -> size_nat
+  -> nat
 let genA_getC cBuf cPos = 
   let subbuffer = Seq.slice (to_lbytes cBuf) (cPos * computed_b) ((cPos+1) * computed_b) in
   nat_from_bytes_le subbuffer
@@ -252,7 +237,7 @@ val genA_while:
   -> cBuf: bytes{Seq.length cBuf < max_size_t /\ Seq.length cBuf >= 2} 
   -> s:nat 
   -> a:polys_t 
-  -> pos: size_nat{(pos+1) * computed_b <= Seq.length cBuf} 
+  -> pos: size_nat
   -> bPrime:size_nat{bPrime >= 1 /\ params_rateXOF * bPrime = Seq.length cBuf} 
   -> i:nat 
   -> fuel:nat 
@@ -263,9 +248,9 @@ let rec genA_while #seedALen seedA cBuf s a pos bPrime i fuel =
   else if i < params_k * params_n
   then 
     let s, pos, bPrime, cBuf =
-      if pos > ((params_rateXOF * bPrime) / computed_b) - 4 then 
+      if pos > ((params_rateXOF * bPrime) / computed_b) - 1 then 
         let s, pos, bPrime = s + 1, 0, 1 in
-        let cBuf = cshake128_qtesla seedALen seedA s (params_rateXOF * bPrime) in
+        let cBuf = params_genA_xof seedALen seedA s (params_rateXOF * bPrime) in
         s, pos, bPrime, cBuf
       else 
         s, pos, bPrime, cBuf 
@@ -295,7 +280,7 @@ val genA_oracle:
 val genA: #seedALen:size_nat -> seedA:lbytes seedALen -> polys_t
 let genA #seedALen seedA =
   let bPrime = params_bGenA in
-  let cBuf = cshake128_frodo seedALen seedA (u16 0) (params_rateXOF * bPrime) in
+  let cBuf = params_genA_xof seedALen seedA 0 (params_rateXOF * bPrime) in
   let i = 0 in
   let pos = 0 in
   let a = create_polys in
@@ -319,7 +304,7 @@ val gaussSampler_doloop3:
 let rec gaussSampler_doloop3 rand nonce fuel =
   assert_norm(bytelen params_xi < max_size_t); // Need to prove this is a size_nat for use with cshake128_frodo.
   if fuel = 0 then None else
-  let y = nat_from_bytes_le (cshake128_qtesla params_kappa rand nonce (bytelen params_xi)) in
+  let y = nat_from_bytes_le (params_gaussSampler_xof params_kappa rand nonce (bytelen params_xi)) in
   let nonce = nonce + 1 in
   if y < params_xi - 1
   then Some (y, nonce)
@@ -346,13 +331,13 @@ val gaussSampler_doloop2: rand: (lbytes params_kappa) -> nonce: positive -> fuel
 let rec gaussSampler_doloop2 rand nonce fuel =
     if fuel = 0 then None else
     let y, nonce = Some?.v (gaussSampler_doloop3 rand nonce (gaussSampler_doloop3_oracle rand nonce)) in
-    let r = nat_from_bytes_le (cshake128_qtesla params_kappa rand nonce (params_w / 8)) in
+    let r = nat_from_bytes_le (params_gaussSampler_xof params_kappa rand nonce (params_w / 8)) in
     let nonce = nonce + 1 in
     let x = 0 in
     let x = gaussSampler_doloop10 r x in
     let z:nat = params_xi * x + y in
     assume(z < params_q); // TODO: Patrick tells us this is true.
-    let r = cshake128_qtesla params_kappa rand nonce (params_w / 8) in
+    let r = params_gaussSampler_xof params_kappa rand nonce (params_w / 8) in
     let nonce = nonce + 1 in
     if (berSampler r (y * (y + 2 * params_xi * x)) = 0)
     then gaussSampler_doloop2 rand nonce (fuel - 1)
@@ -485,8 +470,6 @@ let qTesla_keygen =
   let pk = (seedA, t) in
   sk, pk
 
-let ySampler_XOF = cshake128_qtesla
-
 val ySampler_while: 
     rand: lbytes params_kappa 
   -> cBuf: bytes{Seq.length cBuf < max_size_t /\ Seq.length cBuf >= 2} 
@@ -504,7 +487,7 @@ let rec ySampler_while rand cBuf pos nPrime sPrime i y fuel =
   then let sPrime, pos, nPrime, cBuf =
     if pos >= nPrime 
     then let sPrime, pos, nPrime = sPrime + 1, 0, params_rateXOF / b in
-         let cBuf = ySampler_XOF (Seq.length rand) rand sPrime params_rateXOF in
+         let cBuf = params_ysampler_xof (Seq.length rand) rand sPrime params_rateXOF in
          sPrime, pos, nPrime, cBuf
     else sPrime, pos, nPrime, cBuf in
     let yi = (nat_from_bytes_le (Seq.slice (to_lbytes cBuf) (pos * b) ((pos + 1) * b))) % (pow2 computed_ySampler_modulus) - params_B in
@@ -533,18 +516,18 @@ let ySampler rand nonce =
   let b = computed_ySampler_b in
   let y = create_poly in
   let pos, nPrime, sPrime = 0, params_n, nonce * 256 in
-  let cBuf = ySampler_XOF (Seq.length rand) rand sPrime (b * nPrime) in
+  let cBuf = params_ysampler_xof (Seq.length rand) rand sPrime (b * nPrime) in
   let i = 0 in
   let fuel = ySampler_oracle rand cBuf pos nPrime sPrime i y in
   Some?.v (ySampler_while rand cBuf pos nPrime sPrime i y fuel)
 
 val hashH: 
     #mlen: size_nat{params_k * params_n + mlen <= max_size_t} 
-  -> polys_t 
-  -> lbytes mlen 
+  -> v: polys_t 
+  -> mdig: lbytes mlen{mlen = 64} // 64 is hard-coded in the spec as the output of G provided here.
   -> lbytes params_kappa
-let hashH #mlen v m =
-  let w = Seq.create (params_k * params_n + mlen) (u8 0) in
+let hashH #mlen v mdig =
+  let w = Seq.create (params_k * params_n + 64) (u8 0) in
   let w = Loops.repeati params_k
     (fun i w -> Loops.repeati params_n
       (fun j w -> let vij:field_t = (Seq.index (Seq.index v i) j) in
@@ -564,8 +547,8 @@ let hashH #mlen v m =
       ) w
     ) w in
   let w = Loops.repeati mlen
-    (fun i w -> Seq.upd w (params_k * params_n + i) (*w.[params_k * params_n + i] <- *) (Seq.index m i) (*m.[i]*)) w in
-  let cPrime = params_hash_shake (Seq.length w) w params_kappa in
+    (fun i w -> Seq.upd w (params_k * params_n + i) (Seq.index mdig i)) w in
+  let cPrime = params_hashH_shake (Seq.length w) w params_kappa in
   cPrime
 
 let signlist_elt = x:int{x = -1 \/ x == 1}
@@ -584,17 +567,17 @@ val enc_while:
   -> sign_list: signlist_t 
   -> cnt: size_nat 
   -> c: poly_t 
-  -> s:uint16 
+  -> s: nat
   -> i: size_nat 
-  -> fuel:nat 
+  -> fuel: nat 
   -> Tot (option poly_t) (decreases %[(params_h - i); fuel])
 let rec enc_while cPrime rBuf pos_list sign_list cnt c s i fuel =
   if fuel = 0 then None else
   if i < params_h then 
     let cnt, s, rBuf =
     if cnt > (params_rateXOF - 3)
-    then let s, cnt = add_mod s (u16 1), 0 in // TODO: add_mod ok?
-	 let rBuf = cshake128_frodo params_kappa cPrime s params_rateXOF in
+    then let s, cnt = s + 1, 0 in // TODO: add_mod ok?
+	 let rBuf = params_enc_xof params_kappa cPrime s params_rateXOF in
 	 cnt, s, rBuf
     else cnt, s, rBuf in
   let pos = ((enc_while_getR rBuf cnt) * 256 + (enc_while_getR rBuf (cnt+1))) % params_n in
@@ -610,7 +593,7 @@ let rec enc_while cPrime rBuf pos_list sign_list cnt c s i fuel =
   let cnt = cnt + 3 in
   enc_while cPrime rBuf pos_list sign_list cnt c s i fuel
   else Some c
-	       
+
 assume 
 val enc_oracle: 
     cPrime: (lbytes params_kappa) 
@@ -619,15 +602,15 @@ val enc_oracle:
   -> sign_list: signlist_t 
   -> cnt: size_nat{cnt < params_rateXOF - 2} 
   -> c: poly_t 
-  -> s:uint16 
+  -> s: nat 
   -> i: size_nat 
-  -> Tot (fuel:nat{Some? (enc_while cPrime rBuf pos_list sign_list cnt c s i fuel)})
+  -> Tot (fuel: nat{Some? (enc_while cPrime rBuf pos_list sign_list cnt c s i fuel)})
 
 val enc: lbytes params_kappa -> poly_t
 let enc cPrime =
-  let s = u16 0 in
+  let s = 0 in
   let cnt = 0 in
-  let rBuf = cshake128_frodo params_kappa cPrime s params_rateXOF in
+  let rBuf = params_enc_xof params_kappa cPrime s params_rateXOF in
   let i = 0 in
   let c:poly_t = create_poly in
   let pos_list: Seq.lseq int params_h = Seq.create params_h 0 in
@@ -648,7 +631,7 @@ let intL n =
   mod_pm n (pow2 params_d)
   
 // mod_pm: R_q x Z -> R_q
-val poly_mod_pm: poly_t -> n:nat{n >= 2} -> poly_t
+val poly_mod_pm: poly_t -> n:nat{n >= 2 /\ n <= params_q} -> poly_t
 let poly_mod_pm f n =
   Loops.repeati (Seq.length f)
   (fun i (f:poly_t) ->
@@ -656,10 +639,12 @@ let poly_mod_pm f n =
     Seq.upd f i fi) f
 
 let fnL f = 
+  // These facts about 2^d need to be explicitly proven to satisfy the precondition on poly_mod_pm.
   assert_norm(pow2 params_d >= 2);
+  assert_norm(pow2 params_d <= params_q);
   poly_mod_pm f (pow2 params_d)
 
-#reset-options "--z3rlimit 50 --max_fuel 0"
+#reset-options "--z3rlimit 100 --max_fuel 0"
 
 // [*]_M: Z -> Z
 val intM: c: int -> field_t
@@ -718,6 +703,9 @@ let test_w w =
   (fun i res -> res || 
     (lInfiniteNorm (fnL (Seq.index w i))) >= ((pow2 (params_d - 1)) - params_Le) ||
     (lInfiniteNorm (Seq.index w i)) >= (params_q / 2) - params_Le) res
+
+val hashG: #mlen: size_nat -> m: lbytes mlen -> Tot (lbytes 64)
+let hashG #mlen m = params_hashG mlen m 64
     
 val qtesla_sign_step4: #mLen: size_nat{params_k * params_n + mLen <= max_size_t} -> m: (lbytes mLen) -> sk: qtesla_sk -> r: (lbytes params_kappa) -> rand: (lbytes params_kappa) -> counter:positive -> fuel:nat -> Tot (option qtesla_sig) (decreases fuel)
 let rec qtesla_sign_step4 #mLen m sk r rand counter fuel =
@@ -730,7 +718,7 @@ let rec qtesla_sign_step4 #mLen m sk r rand counter fuel =
     (fun i (v:polys_t) -> 
       let vi:poly_t = ((Seq.index a i) `poly_ntt_mul` y) `poly_mod_pm` params_q in
       Seq.upd v i vi) v in
-  let cPrime = hashH (polysM v) m in
+  let cPrime = hashH (polysM v) (hashG m) in
   let c = enc cPrime in
   let z = y `poly_add` (s `poly_mul` c) in
   if test_rejection z
@@ -759,7 +747,7 @@ let qtesla_sign #mLen m sk =
   let s, e, seedA, seedY = sk in
   let counter = 1 in
   let r = random_bytes params_kappa in
-  let rand = prf2 seedY r m in
+  let rand = prf2 seedY r (hashG m) in
   let fuel = qtesla_sign_oracle m sk r rand counter in
   let res = qtesla_sign_step4 m sk r rand counter fuel in
   Some?.v res
@@ -785,6 +773,6 @@ let qtesla_verify #mLen m sig pk =
       let ti = Seq.index t i in
       let wi = ((ai `poly_ntt_mul` z) `poly_sub` (ti `poly_mul` c)) `poly_mod_pm` params_q in
       Seq.upd w i wi) w in
-  if test_rejection z || not (compare cPrime (hashH (polysM w) m))
+  if test_rejection z || not (compare cPrime (hashH (polysM w) (hashG m)))
   then false
   else true
